TEMP

Risc0/Gadgets/IsZero/Constraints/WeakestPresPart1.lean
@@ -7,36 +7,78 @@ namespace Risc0.IsZero.Constraints.WP
 
 open MLIRNotation
 
--- The state obtained by running Code.part₁ on st
-def part₁_state (st: State) : State := 
-  ((st["x"] ←ₛ getImpl st { name := "input" } 0 0)["out[0]"] ←ₛ
-          getImpl st { name := "output" } 0 0)[props][{ name := "andEqz x" }] ←
-        (Option.get!
-            (State.props
-              ((st["x"] ←ₛ getImpl st { name := "input" } 0 0)["out[0]"] ←ₛ getImpl st { name := "output" } 0 0)
-              { name := "true" }) ∧
-          Option.get! (State.felts (st["x"] ←ₛ getImpl st { name := "input" } 0 0) { name := "x" }) =
-            0)
+-- The state obtained by running Code.part1 on st
+def part1_state (st: State) : State :=
+  
+        ((((st[props][{ name := "%5" : PropVar }] ←
+                (Option.get! (State.props st { name := "%1" : PropVar }) ∧
+                  if Option.get! (State.felts st { name := "%3" : FeltVar }) = (0 : Felt) then True
+                  else Option.get! (State.props st { name := "%4" : PropVar })))[felts][{ name := "%0" : FeltVar }] ←
+              (1 : Felt))[felts][{ name := "%6" : FeltVar }] ←
+            (1 : Felt) - Option.get! (State.felts st { name := "%3" : FeltVar }))["%7"] ←ₛ
+          getImpl st { name := "data" : BufferVar } (0 : Back) (1 : ℕ)) 
 
--- Run the whole program by using part₁_state rather than Code.part₁
-def part₁_state_update (st: State): State :=
-  Γ (part₁_state st) ⟦Code.part₂; Code.part₃; Code.part₄⟧
+def part1_drops (st: State) : State :=
+  State.dropFelts (st) ⟨"%3"⟩
 
--- Prove that substituting part₁_state for Code.part₁ produces the same result
-lemma part₁_wp {st : State} :
-  Code.getReturn (MLIR.runProgram (Code.part₁; Code.part₂; Code.part₃; Code.part₄) st) ↔
-  Code.getReturn (part₁_state_update st) := by
+-- Run the program from part1 onwards by using part1_state rather than Code.part1
+def part1_state_update (st: State): State :=
+  Γ (part1_drops (part1_state st)) ⟦Code.part2;dropfelt ⟨"%2"⟩;dropfelt ⟨"%0"⟩;dropfelt ⟨"%6"⟩;dropfelt ⟨"%7"⟩;dropfelt ⟨"%8"⟩;dropfelt ⟨"%9"⟩⟧
+
+-- Prove that substituting part1_state for Code.part1 produces the same result
+lemma part1_wp {st : State} :
+  Code.getReturn (MLIR.runProgram (Code.part1;dropfelt ⟨"%3"⟩;Code.part2;dropfelt ⟨"%2"⟩;dropfelt ⟨"%0"⟩;dropfelt ⟨"%6"⟩;dropfelt ⟨"%7"⟩;dropfelt ⟨"%8"⟩;dropfelt ⟨"%9"⟩) st) ↔
+  Code.getReturn (part1_state_update st) := by
   unfold MLIR.runProgram; simp only
-  generalize eq : (Code.part₂; Code.part₃; Code.part₄) = prog
-  unfold Code.part₁
+  generalize eq : (dropfelt ⟨"%3"⟩;Code.part2;dropfelt ⟨"%2"⟩;dropfelt ⟨"%0"⟩;dropfelt ⟨"%6"⟩;dropfelt ⟨"%7"⟩;dropfelt ⟨"%8"⟩;dropfelt ⟨"%9"⟩) = prog
+  unfold Code.part1
   MLIR
-  unfold part₁_state_update part₁_state
   rewrite [←eq]
+  rewrite [MLIR.run_seq_def,MLIR.run_dropfelt]
+  unfold part1_state_update part1_drops part1_state
   rfl
 
-lemma part₁_updates_opaque {st : State} : 
-  Code.getReturn (part₀_state_update st) ↔
-  Code.getReturn (part₁_state_update (part₀_state st)) := by
-  simp [part₀_state_update, part₁_wp]
+lemma part1_updates_opaque {st : State} : 
+  Code.getReturn (part0_state_update st) ↔
+  Code.getReturn (part1_state_update (part0_drops (part0_state st))) := by
+  simp [part0_state_update, part1_wp]
+
+lemma part1_cumulative_wp {x0 y0 y1: Felt} :
+  Code.run (start_state [x0] ([y0,y1])) ↔
+  Code.getReturn
+      (part1_state_update
+        (((({
+                  buffers :=
+                    ((fun x => Map.empty x)[{ name := "data" : BufferVar }] ←ₘ
+                        [[some y0, some y1]])[{ name := "in" : BufferVar }] ←ₘ
+                      [[some x0]],
+                  bufferWidths :=
+                    ((fun x => Map.empty x)[{ name := "data" : BufferVar }] ←ₘ (2 : ℕ))[{ name := "in" : BufferVar }] ←ₘ
+                      (1 : ℕ),
+                  constraints := [], cycle := (0 : ℕ), felts := Map.empty, isFailed := false, props := Map.empty,
+                  vars :=
+                    [{ name := "in" : BufferVar },
+                      { name := "data" : BufferVar }] }[props][{ name := "%1" : PropVar }] ←
+                True)[felts][{ name := "%2" : FeltVar }] ←
+              x0)[props][{ name := "%4" : PropVar }] ←
+            x0 = (0 : Felt))[felts][{ name := "%3" : FeltVar }] ←
+          y0))  := by
+    rewrite [part0_cumulative_wp]
+    rewrite [part1_updates_opaque]
+    unfold part0_state
+    MLIR_states_updates
+    -- 0 withEqZeros
+    -- rewrite [withEqZero_def]
+    -- MLIR_states_updates
+    unfold part0_drops
+    -- 0 drops
+    -- simp only [State.drop_update_swap, State.drop_update_same, State.drop_updateProps_swap]
+    -- rewrite [State.dropFelts]
+    -- simp only [State.dropFelts_buffers, State.dropFelts_bufferWidths, State.dropFelts_constraints, State.dropFelts_cycle, State.dropFelts_felts, State.dropFelts_isFailed, State.dropFelts_props, State.dropFelts_vars]
+    -- simp only [Map.drop_base, ne_eq, Map.update_drop_swap, Map.update_drop]
+    -- 0 sets
+    -- rewrite [Map.drop_of_updates]
+    -- simp only [Map.drop_base, ne_eq, Map.update_drop_swap, Map.update_drop]
+    rfl
 
 end Risc0.IsZero.Constraints.WP
