Risc0/Gadgets/IsZero/Witness/WeakestPresPart1.lean
@@ -7,34 +7,92 @@ namespace Risc0.IsZero.Witness.WP
 
 open MLIRNotation
 
--- The state obtained by running Code.part₁ on st
-def part₁_state (st: State) : State :=
-  State.set! (State.updateFelts (State.set! (State.updateFelts st
-    { name := "isZeroBit" }
-    (if Option.get! (State.felts st { name := "x" }) = 0 then 1 else 0)) { name := "output" } 0
-    (if Option.get! (State.felts st { name := "x" }) = 0 then 1 else 0)) { name := "invVal" }
-    (if Option.get! st.felts[({ name := "x" } : FeltVar)]! = 0 then 0 else (Option.get! st.felts[({ name := "x" } : FeltVar)]!)⁻¹)) { name := "output" } 1
-    (if Option.get! st.felts[({ name := "x" } : FeltVar)]! = 0 then 0 else (Option.get! st.felts[({ name := "x" } : FeltVar)]!)⁻¹)
+-- The state obtained by running Code.part1 on st
+def part1_state (st: State) : State :=
+  
+          ((if
+                Option.get!
+                    ((State.set! st { name := "data" : BufferVar } (1 : ℕ)
+                            (Option.get! st.felts[{ name := "%5" : FeltVar }]!))["%2"] ←ₛ
+                          getImpl st { name := "data" : BufferVar } (0 : Back)
+                            (0 : ℕ)).felts[{ name := "%2" : FeltVar }]! =
+                  (0 : Felt) then
+              (State.set! st { name := "data" : BufferVar } (1 : ℕ)
+                  (Option.get! st.felts[{ name := "%5" : FeltVar }]!))["%2"] ←ₛ
+                getImpl st { name := "data" : BufferVar } (0 : Back) (0 : ℕ)
+            else
+              withEqZero
+                (Option.get!
+                  ((State.set! st { name := "data" : BufferVar } (1 : ℕ)
+                          (Option.get! st.felts[{ name := "%5" : FeltVar }]!))["%2"] ←ₛ
+                        getImpl st { name := "data" : BufferVar } (0 : Back)
+                          (0 : ℕ)).felts[{ name := "%1" : FeltVar }]!)
+                ((State.set! st { name := "data" : BufferVar } (1 : ℕ)
+                    (Option.get! st.felts[{ name := "%5" : FeltVar }]!))["%2"] ←ₛ
+                  getImpl st { name := "data" : BufferVar } (0 : Back) (0 : ℕ)))[felts][{ name := "%0" : FeltVar }] ←
+            (1 : Felt)) 
 
--- Run the program from part₁ onwards by using part₁_state rather than Code.part₁
-def part₁_state_update (st: State): State :=
-  Γ (part₁_state st) ⟦Code.part₂; Code.part₃; Code.part₄; Code.part₅⟧
+def part1_drops (st: State) : State :=
+  st
 
--- Prove that substituting part₁_state for Code.part₁ produces the same result
-lemma part₁_wp {st : State} {y₁ y₂ : Option Felt} :
-  (MLIR.runProgram (Code.part₁; Code.part₂; Code.part₃; Code.part₄; Code.part₅) st).lastOutput = [y₁, y₂] ↔
-  (part₁_state_update st).lastOutput = [y₁, y₂] := by
+-- Run the program from part1 onwards by using part1_state rather than Code.part1
+def part1_state_update (st: State): State :=
+  Γ (part1_drops (part1_state st)) ⟦Code.part2;dropfelt ⟨"%1"⟩;dropfelt ⟨"%4"⟩;dropfelt ⟨"%5"⟩;dropfelt ⟨"%2"⟩;dropfelt ⟨"%0"⟩;dropfelt ⟨"%3"⟩;dropfelt ⟨"%6"⟩⟧
+
+-- Prove that substituting part1_state for Code.part1 produces the same result
+lemma part1_wp {st : State} {y0 y1 : Option Felt} :
+  Code.getReturn (MLIR.runProgram (Code.part1;Code.part2;dropfelt ⟨"%1"⟩;dropfelt ⟨"%4"⟩;dropfelt ⟨"%5"⟩;dropfelt ⟨"%2"⟩;dropfelt ⟨"%0"⟩;dropfelt ⟨"%3"⟩;dropfelt ⟨"%6"⟩) st) = [y0, y1] ↔
+  Code.getReturn (part1_state_update st) = [y0, y1] := by
   unfold MLIR.runProgram; simp only
-  generalize eq : (Code.part₂; Code.part₃; Code.part₄; Code.part₅) = prog
-  unfold Code.part₁
+  generalize eq : (Code.part2;dropfelt ⟨"%1"⟩;dropfelt ⟨"%4"⟩;dropfelt ⟨"%5"⟩;dropfelt ⟨"%2"⟩;dropfelt ⟨"%0"⟩;dropfelt ⟨"%3"⟩;dropfelt ⟨"%6"⟩) = prog
+  unfold Code.part1
   MLIR
   rewrite [←eq]
-  unfold part₁_state_update part₁_state
+  
+  unfold part1_state_update part1_drops part1_state
   rfl
 
-lemma part₁_updates_opaque {st : State} : 
-  (part₀_state_update st).lastOutput = [y₁, y₂] ↔
-  (part₁_state_update (part₀_state st)).lastOutput = [y₁, y₂] := by
-  simp [part₀_state_update, part₁_wp]
+lemma part1_updates_opaque {st : State} : 
+  Code.getReturn (part0_state_update st) = [y0, y1] ↔
+  Code.getReturn (part1_state_update (part0_drops (part0_state st))) = [y0, y1] := by
+  simp [part0_state_update, part1_wp]
+
+lemma part1_cumulative_wp {x0: Felt} :
+  Code.run (start_state [x0]) = [y0,y1] ↔
+  Code.getReturn
+        (part1_state_update
+          ({
+              buffers :=
+                (Map.empty[{ name := "in" : BufferVar }] ←ₘ [[some x0]])[{ name := "data" : BufferVar }] ←ₘ
+                  [[some (if x0 = (0 : Felt) then (1 : Felt) else (0 : Felt)), none]],
+              bufferWidths :=
+                ((fun x => Map.empty x)[{ name := "data" : BufferVar }] ←ₘ (2 : ℕ))[{ name := "in" : BufferVar }] ←ₘ
+                  (1 : ℕ),
+              constraints := [], cycle := (0 : ℕ),
+              felts :=
+                ((fun x => Map.empty x)[{ name := "%1" : FeltVar }] ←ₘ x0)[{ name := "%4" : FeltVar }] ←ₘ
+                  if x0 = (0 : Felt) then (1 : Felt) else (0 : Felt),
+              isFailed := false, props := Map.empty,
+              vars :=
+                [{ name := "in" : BufferVar }, { name := "data" : BufferVar }] }[felts][{ name := "%5" : FeltVar }] ←
+            if x0 = (0 : Felt) then (0 : Felt) else x0⁻¹)) =
+      [y0, y1]  := by
+    rewrite [part0_cumulative_wp]
+    rewrite [part1_updates_opaque]
+    unfold part0_state
+    try simplify_get_hack
+    MLIR_states_updates
+    -- 0 withEqZeros
+    -- rewrite [withEqZero_def]
+    -- MLIR_states_updates
+    unfold part0_drops
+    -- 0 drops
+    -- simp only [State.drop_update_swap, State.drop_update_same]
+    -- rewrite [State.dropFelts]
+    -- simp only [State.dropFelts_buffers, State.dropFelts_bufferWidths, State.dropFelts_constraints, State.dropFelts_cycle, State.dropFelts_felts, State.dropFelts_isFailed, State.dropFelts_props, State.dropFelts_vars]
+    -- simp only [Map.drop_base, ne_eq, Map.update_drop_swap, Map.update_drop]
+    -- 1 set
+    rewrite [Map.drop_of_updates]
+    simp only [Map.drop_base, ne_eq, Map.update_drop_swap, Map.update_drop]
 
 end Risc0.IsZero.Witness.WP
