Risc0/Gadgets/IsZero/Witness/WeakestPresPart2.lean
@@ -7,29 +7,912 @@ namespace Risc0.IsZero.Witness.WP
 
 open MLIRNotation
 
--- The state obtained by running Code.part₂ on st
-def part₂_state (st: State) : State :=
-  st["arg1[0]"] ←ₛ getImpl st { name := "output" } 0 0
+-- The state obtained by running Code.part2 on st
+def part2_state (st: State) : State :=
+  
+          (if
+              Option.get! (State.felts st { name := "%0" : FeltVar }) -
+                  Option.get! (State.felts st { name := "%2" : FeltVar }) =
+                (0 : Felt) then
+            st[felts][{ name := "%3" : FeltVar }] ←
+              Option.get! (State.felts st { name := "%0" : FeltVar }) -
+                Option.get! (State.felts st { name := "%2" : FeltVar })
+          else
+            withEqZero
+              (Option.get! (State.felts st { name := "%1" : FeltVar }) *
+                  Option.get!
+                    (State.felts
+                      ((st[felts][{ name := "%3" : FeltVar }] ←
+                          Option.get! (State.felts st { name := "%0" : FeltVar }) -
+                            Option.get! (State.felts st { name := "%2" : FeltVar }))["%4"] ←ₛ
+                        getImpl st { name := "data" : BufferVar } (0 : Back) (1 : ℕ))
+                      { name := "%4" : FeltVar }) -
+                Option.get! (State.felts st { name := "%0" : FeltVar }))
+              ((((st[felts][{ name := "%3" : FeltVar }] ←
+                      Option.get! (State.felts st { name := "%0" : FeltVar }) -
+                        Option.get! (State.felts st { name := "%2" : FeltVar }))["%4"] ←ₛ
+                    getImpl st { name := "data" : BufferVar } (0 : Back) (1 : ℕ))[felts][{ name := "%5" : FeltVar }] ←
+                  Option.get! (State.felts st { name := "%1" : FeltVar }) *
+                    Option.get!
+                      (State.felts
+                        ((st[felts][{ name := "%3" : FeltVar }] ←
+                            Option.get! (State.felts st { name := "%0" : FeltVar }) -
+                              Option.get! (State.felts st { name := "%2" : FeltVar }))["%4"] ←ₛ
+                          getImpl st { name := "data" : BufferVar } (0 : Back) (1 : ℕ))
+                        { name := "%4" : FeltVar }))[felts][{ name := "%6" : FeltVar }] ←
+                Option.get! (State.felts st { name := "%1" : FeltVar }) *
+                    Option.get!
+                      (State.felts
+                        ((st[felts][{ name := "%3" : FeltVar }] ←
+                            Option.get! (State.felts st { name := "%0" : FeltVar }) -
+                              Option.get! (State.felts st { name := "%2" : FeltVar }))["%4"] ←ₛ
+                          getImpl st { name := "data" : BufferVar } (0 : Back) (1 : ℕ))
+                        { name := "%4" : FeltVar }) -
+                  Option.get! (State.felts st { name := "%0" : FeltVar }))) 
 
--- Run the program from part₂ onwards by using part₂_state rather than Code.part₂
-def part₂_state_update (st: State): State :=
-  Γ (part₂_state st) ⟦Code.part₃; Code.part₄; Code.part₅⟧
+def part2_drops (st: State) : State :=
+  State.dropFelts (State.dropFelts (State.dropFelts (State.dropFelts (State.dropFelts (State.dropFelts (State.dropFelts (st) ⟨"%1"⟩) ⟨"%4"⟩) ⟨"%5"⟩) ⟨"%2"⟩) ⟨"%0"⟩) ⟨"%3"⟩) ⟨"%6"⟩
 
--- Prove that substituting part₂_state for Code.part₂ produces the same result
-lemma part₂_wp {st : State} {y₁ y₂ : Option Felt} :
-  (MLIR.runProgram (Code.part₂; Code.part₃; Code.part₄; Code.part₅) st).lastOutput = [y₁, y₂] ↔
-  (part₂_state_update st).lastOutput = [y₁, y₂] := by
+-- Run the program from part2 onwards by using part2_state rather than Code.part2
+def part2_state_update (st: State): State :=
+  part2_drops (part2_state st)
+
+-- Prove that substituting part2_state for Code.part2 produces the same result
+lemma part2_wp {st : State} {y0 y1 : Option Felt} :
+  Code.getReturn (MLIR.runProgram (Code.part2;dropfelt ⟨"%1"⟩;dropfelt ⟨"%4"⟩;dropfelt ⟨"%5"⟩;dropfelt ⟨"%2"⟩;dropfelt ⟨"%0"⟩;dropfelt ⟨"%3"⟩;dropfelt ⟨"%6"⟩) st) = [y0, y1] ↔
+  Code.getReturn (part2_state_update st) = [y0, y1] := by
   unfold MLIR.runProgram; simp only
-  generalize eq : (Code.part₃; Code.part₄; Code.part₅) = prog
-  unfold Code.part₂
+  generalize eq : (dropfelt ⟨"%1"⟩;dropfelt ⟨"%4"⟩;dropfelt ⟨"%5"⟩;dropfelt ⟨"%2"⟩;dropfelt ⟨"%0"⟩;dropfelt ⟨"%3"⟩;dropfelt ⟨"%6"⟩) = prog
+  unfold Code.part2
   MLIR
   rewrite [←eq]
-  unfold part₂_state_update part₂_state
+  rewrite [MLIR.run_seq_def,MLIR.run_dropfelt, MLIR.run_seq_def,MLIR.run_dropfelt, MLIR.run_seq_def,MLIR.run_dropfelt, MLIR.run_seq_def,MLIR.run_dropfelt, MLIR.run_seq_def,MLIR.run_dropfelt, MLIR.run_seq_def,MLIR.run_dropfelt, MLIR.run_dropfelt]
+  unfold part2_state_update part2_drops part2_state
   rfl
 
-lemma part₂_updates_opaque {st : State} : 
-  (part₁_state_update st).lastOutput = [y₁, y₂] ↔
-  (part₂_state_update (part₁_state st)).lastOutput = [y₁, y₂] := by
-  simp [part₁_state_update, part₂_wp]
+lemma part2_updates_opaque {st : State} : 
+  Code.getReturn (part1_state_update st) = [y0, y1] ↔
+  Code.getReturn (part2_state_update (part1_drops (part1_state st))) = [y0, y1] := by
+  simp [part1_state_update, part2_wp]
 
+lemma part2_cumulative_wp {x0: Felt} :
+  Code.run (start_state [x0]) = [y0,y1] ↔
+  Code.getReturn
+        (part2_state_update
+          ((if (if x0 = (0 : Felt) then (1 : Felt) else (0 : Felt)) = (0 : Felt) then
+              {
+                  buffers :=
+                    (Map.empty[{ name := "in" : BufferVar }] ←ₘ [[some x0]])[{ name := "data" : BufferVar }] ←ₘ
+                      [[some (if x0 = (0 : Felt) then (1 : Felt) else (0 : Felt)),
+                          some (if x0 = (0 : Felt) then (0 : Felt) else x0⁻¹)]],
+                  bufferWidths :=
+                    ((fun x => Map.empty x)[{ name := "data" : BufferVar }] ←ₘ (2 : ℕ))[{ name := "in" : BufferVar }] ←ₘ
+                      (1 : ℕ),
+                  constraints := [], cycle := (0 : ℕ),
+                  felts :=
+                    (((fun x => Map.empty x)[{ name := "%1" : FeltVar }] ←ₘ x0)[{ name := "%4" : FeltVar }] ←ₘ
+                        if x0 = (0 : Felt) then (1 : Felt) else (0 : Felt))[{ name := "%5" : FeltVar }] ←ₘ
+                      if x0 = (0 : Felt) then (0 : Felt) else x0⁻¹,
+                  isFailed := false, props := Map.empty,
+                  vars :=
+                    [{ name := "in" : BufferVar },
+                      { name := "data" : BufferVar }] }[felts][{ name := "%2" : FeltVar }] ←
+                if x0 = (0 : Felt) then (1 : Felt) else (0 : Felt)
+            else
+              withEqZero x0
+                ({
+                    buffers :=
+                      (Map.empty[{ name := "in" : BufferVar }] ←ₘ [[some x0]])[{ name := "data" : BufferVar }] ←ₘ
+                        [[some (if x0 = (0 : Felt) then (1 : Felt) else (0 : Felt)),
+                            some (if x0 = (0 : Felt) then (0 : Felt) else x0⁻¹)]],
+                    bufferWidths :=
+                      ((fun x => Map.empty x)[{ name := "data" : BufferVar }] ←ₘ
+                          (2 : ℕ))[{ name := "in" : BufferVar }] ←ₘ
+                        (1 : ℕ),
+                    constraints := [], cycle := (0 : ℕ),
+                    felts :=
+                      (((fun x => Map.empty x)[{ name := "%1" : FeltVar }] ←ₘ x0)[{ name := "%4" : FeltVar }] ←ₘ
+                          if x0 = (0 : Felt) then (1 : Felt) else (0 : Felt))[{ name := "%5" : FeltVar }] ←ₘ
+                        if x0 = (0 : Felt) then (0 : Felt) else x0⁻¹,
+                    isFailed := false, props := Map.empty,
+                    vars :=
+                      [{ name := "in" : BufferVar },
+                        { name := "data" : BufferVar }] }[felts][{ name := "%2" : FeltVar }] ←
+                  if x0 = (0 : Felt) then (1 : Felt) else (0 : Felt)))[felts][{ name := "%0" : FeltVar }] ←
+            (1 : Felt))) =
+      [y0, y1]  := by
+    rewrite [part1_cumulative_wp]
+    rewrite [part2_updates_opaque]
+    unfold part1_state
+    try simplify_get_hack
+    MLIR_states_updates
+    -- 0 withEqZeros
+    -- rewrite [withEqZero_def]
+    -- MLIR_states_updates
+    unfold part1_drops
+    -- 0 drops
+    -- simp only [State.drop_update_swap, State.drop_update_same]
+    -- rewrite [State.dropFelts]
+    -- simp only [State.dropFelts_buffers, State.dropFelts_bufferWidths, State.dropFelts_constraints, State.dropFelts_cycle, State.dropFelts_felts, State.dropFelts_isFailed, State.dropFelts_props, State.dropFelts_vars]
+    -- simp only [Map.drop_base, ne_eq, Map.update_drop_swap, Map.update_drop]
+    -- 1 set
+    rewrite [Map.drop_of_updates]
+    simp only [Map.drop_base, ne_eq, Map.update_drop_swap, Map.update_drop]
+
+lemma closed_form {x0: Felt} :
+  Code.run (start_state [x0]) = [y0,y1] ↔
+   (match
+        Option.get!
+          (State.buffers
+            (if ((1 : Felt) - if x0 = (0 : Felt) then (1 : Felt) else (0 : Felt)) = (0 : Felt) then
+              ((if x0 = (0 : Felt) → False then
+                    {
+                        buffers :=
+                          ((fun x => Map.empty x)[{ name := "in" : BufferVar }] ←ₘ
+                              [[some x0]])[{ name := "data" : BufferVar }] ←ₘ
+                            [[some (if x0 = (0 : Felt) then (1 : Felt) else (0 : Felt)),
+                                some (if x0 = (0 : Felt) then (0 : Felt) else x0⁻¹)]],
+                        bufferWidths :=
+                          ((fun x => Map.empty x)[{ name := "data" : BufferVar }] ←ₘ
+                              (2 : ℕ))[{ name := "in" : BufferVar }] ←ₘ
+                            (1 : ℕ),
+                        constraints := [], cycle := (0 : ℕ),
+                        felts :=
+                          (((fun x => Map.empty x)[{ name := "%1" : FeltVar }] ←ₘ x0)[{ name := "%4" : FeltVar }] ←ₘ
+                              if x0 = (0 : Felt) then (1 : Felt) else (0 : Felt))[{ name := "%5" : FeltVar }] ←ₘ
+                            if x0 = (0 : Felt) then (0 : Felt) else x0⁻¹,
+                        isFailed := false, props := Map.empty,
+                        vars :=
+                          [{ name := "in" : BufferVar },
+                            { name := "data" : BufferVar }] }[felts][{ name := "%2" : FeltVar }] ←
+                      if x0 = (0 : Felt) then (1 : Felt) else (0 : Felt)
+                  else
+                    withEqZero x0
+                      ({
+                          buffers :=
+                            ((fun x => Map.empty x)[{ name := "in" : BufferVar }] ←ₘ
+                                [[some x0]])[{ name := "data" : BufferVar }] ←ₘ
+                              [[some (if x0 = (0 : Felt) then (1 : Felt) else (0 : Felt)),
+                                  some (if x0 = (0 : Felt) then (0 : Felt) else x0⁻¹)]],
+                          bufferWidths :=
+                            ((fun x => Map.empty x)[{ name := "data" : BufferVar }] ←ₘ
+                                (2 : ℕ))[{ name := "in" : BufferVar }] ←ₘ
+                              (1 : ℕ),
+                          constraints := [], cycle := (0 : ℕ),
+                          felts :=
+                            (((fun x => Map.empty x)[{ name := "%1" : FeltVar }] ←ₘ x0)[{ name := "%4" : FeltVar }] ←ₘ
+                                if x0 = (0 : Felt) then (1 : Felt) else (0 : Felt))[{ name := "%5" : FeltVar }] ←ₘ
+                              if x0 = (0 : Felt) then (0 : Felt) else x0⁻¹,
+                          isFailed := false, props := Map.empty,
+                          vars :=
+                            [{ name := "in" : BufferVar },
+                              { name := "data" : BufferVar }] }[felts][{ name := "%2" : FeltVar }] ←
+                        if x0 = (0 : Felt) then (1 : Felt) else (0 : Felt)))[felts][{ name := "%0" : FeltVar }] ←
+                  (1 : Felt))[felts][{ name := "%3" : FeltVar }] ←
+                (1 : Felt) - if x0 = (0 : Felt) then (1 : Felt) else (0 : Felt)
+            else
+              withEqZero
+                ((x0 *
+                    match
+                      List.get!
+                        (List.get!
+                          (match
+                            State.buffers
+                              (if x0 = (0 : Felt) → False then
+                                {
+                                    buffers :=
+                                      ((fun x => Map.empty x)[{ name := "in" : BufferVar }] ←ₘ
+                                          [[some x0]])[{ name := "data" : BufferVar }] ←ₘ
+                                        [[some (if x0 = (0 : Felt) then (1 : Felt) else (0 : Felt)),
+                                            some (if x0 = (0 : Felt) then (0 : Felt) else x0⁻¹)]],
+                                    bufferWidths :=
+                                      ((fun x => Map.empty x)[{ name := "data" : BufferVar }] ←ₘ
+                                          (2 : ℕ))[{ name := "in" : BufferVar }] ←ₘ
+                                        (1 : ℕ),
+                                    constraints := [], cycle := (0 : ℕ),
+                                    felts :=
+                                      (((fun x => Map.empty x)[{ name := "%1" : FeltVar }] ←ₘ
+                                            x0)[{ name := "%4" : FeltVar }] ←ₘ
+                                          if x0 = (0 : Felt) then (1 : Felt)
+                                          else (0 : Felt))[{ name := "%5" : FeltVar }] ←ₘ
+                                        if x0 = (0 : Felt) then (0 : Felt) else x0⁻¹,
+                                    isFailed := false, props := Map.empty,
+                                    vars :=
+                                      [{ name := "in" : BufferVar },
+                                        { name := "data" : BufferVar }] }[felts][{ name := "%2" : FeltVar }] ←
+                                  if x0 = (0 : Felt) then (1 : Felt) else (0 : Felt)
+                              else
+                                withEqZero x0
+                                  ({
+                                      buffers :=
+                                        ((fun x => Map.empty x)[{ name := "in" : BufferVar }] ←ₘ
+                                            [[some x0]])[{ name := "data" : BufferVar }] ←ₘ
+                                          [[some (if x0 = (0 : Felt) then (1 : Felt) else (0 : Felt)),
+                                              some (if x0 = (0 : Felt) then (0 : Felt) else x0⁻¹)]],
+                                      bufferWidths :=
+                                        ((fun x => Map.empty x)[{ name := "data" : BufferVar }] ←ₘ
+                                            (2 : ℕ))[{ name := "in" : BufferVar }] ←ₘ
+                                          (1 : ℕ),
+                                      constraints := [], cycle := (0 : ℕ),
+                                      felts :=
+                                        (((fun x => Map.empty x)[{ name := "%1" : FeltVar }] ←ₘ
+                                              x0)[{ name := "%4" : FeltVar }] ←ₘ
+                                            if x0 = (0 : Felt) then (1 : Felt)
+                                            else (0 : Felt))[{ name := "%5" : FeltVar }] ←ₘ
+                                          if x0 = (0 : Felt) then (0 : Felt) else x0⁻¹,
+                                      isFailed := false, props := Map.empty,
+                                      vars :=
+                                        [{ name := "in" : BufferVar },
+                                          { name := "data" : BufferVar }] }[felts][{ name := "%2" : FeltVar }] ←
+                                    if x0 = (0 : Felt) then (1 : Felt) else (0 : Felt)))
+                              { name := "data" : BufferVar } with
+                          | some x => x
+                          | none =>
+                            panicWithPosWithDecl "Init.Data.Option.BasicAux" "Option.get!" (16 : ℕ) (14 : ℕ)
+                              "value is none")
+                          (Buffer.Idx.time
+                            ((if x0 = (0 : Felt) → False then
+                                    {
+                                        buffers :=
+                                          ((fun x => Map.empty x)[{ name := "in" : BufferVar }] ←ₘ
+                                              [[some x0]])[{ name := "data" : BufferVar }] ←ₘ
+                                            [[some (if x0 = (0 : Felt) then (1 : Felt) else (0 : Felt)),
+                                                some (if x0 = (0 : Felt) then (0 : Felt) else x0⁻¹)]],
+                                        bufferWidths :=
+                                          ((fun x => Map.empty x)[{ name := "data" : BufferVar }] ←ₘ
+                                              (2 : ℕ))[{ name := "in" : BufferVar }] ←ₘ
+                                            (1 : ℕ),
+                                        constraints := [], cycle := (0 : ℕ),
+                                        felts :=
+                                          (((fun x => Map.empty x)[{ name := "%1" : FeltVar }] ←ₘ
+                                                x0)[{ name := "%4" : FeltVar }] ←ₘ
+                                              if x0 = (0 : Felt) then (1 : Felt)
+                                              else (0 : Felt))[{ name := "%5" : FeltVar }] ←ₘ
+                                            if x0 = (0 : Felt) then (0 : Felt) else x0⁻¹,
+                                        isFailed := false, props := Map.empty,
+                                        vars :=
+                                          [{ name := "in" : BufferVar },
+                                            { name := "data" : BufferVar }] }[felts][{ name := "%2" : FeltVar }] ←
+                                      if x0 = (0 : Felt) then (1 : Felt) else (0 : Felt)
+                                  else
+                                    withEqZero x0
+                                      ({
+                                          buffers :=
+                                            ((fun x => Map.empty x)[{ name := "in" : BufferVar }] ←ₘ
+                                                [[some x0]])[{ name := "data" : BufferVar }] ←ₘ
+                                              [[some (if x0 = (0 : Felt) then (1 : Felt) else (0 : Felt)),
+                                                  some (if x0 = (0 : Felt) then (0 : Felt) else x0⁻¹)]],
+                                          bufferWidths :=
+                                            ((fun x => Map.empty x)[{ name := "data" : BufferVar }] ←ₘ
+                                                (2 : ℕ))[{ name := "in" : BufferVar }] ←ₘ
+                                              (1 : ℕ),
+                                          constraints := [], cycle := (0 : ℕ),
+                                          felts :=
+                                            (((fun x => Map.empty x)[{ name := "%1" : FeltVar }] ←ₘ
+                                                  x0)[{ name := "%4" : FeltVar }] ←ₘ
+                                                if x0 = (0 : Felt) then (1 : Felt)
+                                                else (0 : Felt))[{ name := "%5" : FeltVar }] ←ₘ
+                                              if x0 = (0 : Felt) then (0 : Felt) else x0⁻¹,
+                                          isFailed := false, props := Map.empty,
+                                          vars :=
+                                            [{ name := "in" : BufferVar },
+                                              { name := "data" : BufferVar }] }[felts][{ name := "%2" : FeltVar }] ←
+                                        if x0 = (0 : Felt) then (1 : Felt) else (0 : Felt))).cycle -
+                                Back.toNat (0 : Back),
+                              (1 : ℕ))))
+                        (Buffer.Idx.data
+                          ((if x0 = (0 : Felt) → False then
+                                  {
+                                      buffers :=
+                                        ((fun x => Map.empty x)[{ name := "in" : BufferVar }] ←ₘ
+                                            [[some x0]])[{ name := "data" : BufferVar }] ←ₘ
+                                          [[some (if x0 = (0 : Felt) then (1 : Felt) else (0 : Felt)),
+                                              some (if x0 = (0 : Felt) then (0 : Felt) else x0⁻¹)]],
+                                      bufferWidths :=
+                                        ((fun x => Map.empty x)[{ name := "data" : BufferVar }] ←ₘ
+                                            (2 : ℕ))[{ name := "in" : BufferVar }] ←ₘ
+                                          (1 : ℕ),
+                                      constraints := [], cycle := (0 : ℕ),
+                                      felts :=
+                                        (((fun x => Map.empty x)[{ name := "%1" : FeltVar }] ←ₘ
+                                              x0)[{ name := "%4" : FeltVar }] ←ₘ
+                                            if x0 = (0 : Felt) then (1 : Felt)
+                                            else (0 : Felt))[{ name := "%5" : FeltVar }] ←ₘ
+                                          if x0 = (0 : Felt) then (0 : Felt) else x0⁻¹,
+                                      isFailed := false, props := Map.empty,
+                                      vars :=
+                                        [{ name := "in" : BufferVar },
+                                          { name := "data" : BufferVar }] }[felts][{ name := "%2" : FeltVar }] ←
+                                    if x0 = (0 : Felt) then (1 : Felt) else (0 : Felt)
+                                else
+                                  withEqZero x0
+                                    ({
+                                        buffers :=
+                                          ((fun x => Map.empty x)[{ name := "in" : BufferVar }] ←ₘ
+                                              [[some x0]])[{ name := "data" : BufferVar }] ←ₘ
+                                            [[some (if x0 = (0 : Felt) then (1 : Felt) else (0 : Felt)),
+                                                some (if x0 = (0 : Felt) then (0 : Felt) else x0⁻¹)]],
+                                        bufferWidths :=
+                                          ((fun x => Map.empty x)[{ name := "data" : BufferVar }] ←ₘ
+                                              (2 : ℕ))[{ name := "in" : BufferVar }] ←ₘ
+                                            (1 : ℕ),
+                                        constraints := [], cycle := (0 : ℕ),
+                                        felts :=
+                                          (((fun x => Map.empty x)[{ name := "%1" : FeltVar }] ←ₘ
+                                                x0)[{ name := "%4" : FeltVar }] ←ₘ
+                                              if x0 = (0 : Felt) then (1 : Felt)
+                                              else (0 : Felt))[{ name := "%5" : FeltVar }] ←ₘ
+                                            if x0 = (0 : Felt) then (0 : Felt) else x0⁻¹,
+                                        isFailed := false, props := Map.empty,
+                                        vars :=
+                                          [{ name := "in" : BufferVar },
+                                            { name := "data" : BufferVar }] }[felts][{ name := "%2" : FeltVar }] ←
+                                      if x0 = (0 : Felt) then (1 : Felt) else (0 : Felt))).cycle -
+                              Back.toNat (0 : Back),
+                            (1 : ℕ))) with
+                    | some x => x
+                    | none =>
+                      panicWithPosWithDecl "Init.Data.Option.BasicAux" "Option.get!" (16 : ℕ) (14 : ℕ)
+                        "value is none") -
+                  (1 : Felt))
+                ((((((if x0 = (0 : Felt) → False then
+                            {
+                                buffers :=
+                                  ((fun x => Map.empty x)[{ name := "in" : BufferVar }] ←ₘ
+                                      [[some x0]])[{ name := "data" : BufferVar }] ←ₘ
+                                    [[some (if x0 = (0 : Felt) then (1 : Felt) else (0 : Felt)),
+                                        some (if x0 = (0 : Felt) then (0 : Felt) else x0⁻¹)]],
+                                bufferWidths :=
+                                  ((fun x => Map.empty x)[{ name := "data" : BufferVar }] ←ₘ
+                                      (2 : ℕ))[{ name := "in" : BufferVar }] ←ₘ
+                                    (1 : ℕ),
+                                constraints := [], cycle := (0 : ℕ),
+                                felts :=
+                                  (((fun x => Map.empty x)[{ name := "%1" : FeltVar }] ←ₘ
+                                        x0)[{ name := "%4" : FeltVar }] ←ₘ
+                                      if x0 = (0 : Felt) then (1 : Felt) else (0 : Felt))[{ name := "%5" : FeltVar }] ←ₘ
+                                    if x0 = (0 : Felt) then (0 : Felt) else x0⁻¹,
+                                isFailed := false, props := Map.empty,
+                                vars :=
+                                  [{ name := "in" : BufferVar },
+                                    { name := "data" : BufferVar }] }[felts][{ name := "%2" : FeltVar }] ←
+                              if x0 = (0 : Felt) then (1 : Felt) else (0 : Felt)
+                          else
+                            withEqZero x0
+                              ({
+                                  buffers :=
+                                    ((fun x => Map.empty x)[{ name := "in" : BufferVar }] ←ₘ
+                                        [[some x0]])[{ name := "data" : BufferVar }] ←ₘ
+                                      [[some (if x0 = (0 : Felt) then (1 : Felt) else (0 : Felt)),
+                                          some (if x0 = (0 : Felt) then (0 : Felt) else x0⁻¹)]],
+                                  bufferWidths :=
+                                    ((fun x => Map.empty x)[{ name := "data" : BufferVar }] ←ₘ
+                                        (2 : ℕ))[{ name := "in" : BufferVar }] ←ₘ
+                                      (1 : ℕ),
+                                  constraints := [], cycle := (0 : ℕ),
+                                  felts :=
+                                    (((fun x => Map.empty x)[{ name := "%1" : FeltVar }] ←ₘ
+                                          x0)[{ name := "%4" : FeltVar }] ←ₘ
+                                        if x0 = (0 : Felt) then (1 : Felt)
+                                        else (0 : Felt))[{ name := "%5" : FeltVar }] ←ₘ
+                                      if x0 = (0 : Felt) then (0 : Felt) else x0⁻¹,
+                                  isFailed := false, props := Map.empty,
+                                  vars :=
+                                    [{ name := "in" : BufferVar },
+                                      { name := "data" : BufferVar }] }[felts][{ name := "%2" : FeltVar }] ←
+                                if x0 = (0 : Felt) then (1 : Felt)
+                                else (0 : Felt)))[felts][{ name := "%0" : FeltVar }] ←
+                          (1 : Felt))[felts][{ name := "%3" : FeltVar }] ←
+                        (1 : Felt) -
+                          if x0 = (0 : Felt) then (1 : Felt) else (0 : Felt))[felts][{ name := "%4" : FeltVar }] ←
+                      match
+                        List.get!
+                          (List.get!
+                            (match
+                              State.buffers
+                                (if x0 = (0 : Felt) → False then
+                                  {
+                                      buffers :=
+                                        ((fun x => Map.empty x)[{ name := "in" : BufferVar }] ←ₘ
+                                            [[some x0]])[{ name := "data" : BufferVar }] ←ₘ
+                                          [[some (if x0 = (0 : Felt) then (1 : Felt) else (0 : Felt)),
+                                              some (if x0 = (0 : Felt) then (0 : Felt) else x0⁻¹)]],
+                                      bufferWidths :=
+                                        ((fun x => Map.empty x)[{ name := "data" : BufferVar }] ←ₘ
+                                            (2 : ℕ))[{ name := "in" : BufferVar }] ←ₘ
+                                          (1 : ℕ),
+                                      constraints := [], cycle := (0 : ℕ),
+                                      felts :=
+                                        (((fun x => Map.empty x)[{ name := "%1" : FeltVar }] ←ₘ
+                                              x0)[{ name := "%4" : FeltVar }] ←ₘ
+                                            if x0 = (0 : Felt) then (1 : Felt)
+                                            else (0 : Felt))[{ name := "%5" : FeltVar }] ←ₘ
+                                          if x0 = (0 : Felt) then (0 : Felt) else x0⁻¹,
+                                      isFailed := false, props := Map.empty,
+                                      vars :=
+                                        [{ name := "in" : BufferVar },
+                                          { name := "data" : BufferVar }] }[felts][{ name := "%2" : FeltVar }] ←
+                                    if x0 = (0 : Felt) then (1 : Felt) else (0 : Felt)
+                                else
+                                  withEqZero x0
+                                    ({
+                                        buffers :=
+                                          ((fun x => Map.empty x)[{ name := "in" : BufferVar }] ←ₘ
+                                              [[some x0]])[{ name := "data" : BufferVar }] ←ₘ
+                                            [[some (if x0 = (0 : Felt) then (1 : Felt) else (0 : Felt)),
+                                                some (if x0 = (0 : Felt) then (0 : Felt) else x0⁻¹)]],
+                                        bufferWidths :=
+                                          ((fun x => Map.empty x)[{ name := "data" : BufferVar }] ←ₘ
+                                              (2 : ℕ))[{ name := "in" : BufferVar }] ←ₘ
+                                            (1 : ℕ),
+                                        constraints := [], cycle := (0 : ℕ),
+                                        felts :=
+                                          (((fun x => Map.empty x)[{ name := "%1" : FeltVar }] ←ₘ
+                                                x0)[{ name := "%4" : FeltVar }] ←ₘ
+                                              if x0 = (0 : Felt) then (1 : Felt)
+                                              else (0 : Felt))[{ name := "%5" : FeltVar }] ←ₘ
+                                            if x0 = (0 : Felt) then (0 : Felt) else x0⁻¹,
+                                        isFailed := false, props := Map.empty,
+                                        vars :=
+                                          [{ name := "in" : BufferVar },
+                                            { name := "data" : BufferVar }] }[felts][{ name := "%2" : FeltVar }] ←
+                                      if x0 = (0 : Felt) then (1 : Felt) else (0 : Felt)))
+                                { name := "data" : BufferVar } with
+                            | some x => x
+                            | none =>
+                              panicWithPosWithDecl "Init.Data.Option.BasicAux" "Option.get!" (16 : ℕ) (14 : ℕ)
+                                "value is none")
+                            (Buffer.Idx.time
+                              ((if x0 = (0 : Felt) → False then
+                                      {
+                                          buffers :=
+                                            ((fun x => Map.empty x)[{ name := "in" : BufferVar }] ←ₘ
+                                                [[some x0]])[{ name := "data" : BufferVar }] ←ₘ
+                                              [[some (if x0 = (0 : Felt) then (1 : Felt) else (0 : Felt)),
+                                                  some (if x0 = (0 : Felt) then (0 : Felt) else x0⁻¹)]],
+                                          bufferWidths :=
+                                            ((fun x => Map.empty x)[{ name := "data" : BufferVar }] ←ₘ
+                                                (2 : ℕ))[{ name := "in" : BufferVar }] ←ₘ
+                                              (1 : ℕ),
+                                          constraints := [], cycle := (0 : ℕ),
+                                          felts :=
+                                            (((fun x => Map.empty x)[{ name := "%1" : FeltVar }] ←ₘ
+                                                  x0)[{ name := "%4" : FeltVar }] ←ₘ
+                                                if x0 = (0 : Felt) then (1 : Felt)
+                                                else (0 : Felt))[{ name := "%5" : FeltVar }] ←ₘ
+                                              if x0 = (0 : Felt) then (0 : Felt) else x0⁻¹,
+                                          isFailed := false, props := Map.empty,
+                                          vars :=
+                                            [{ name := "in" : BufferVar },
+                                              { name := "data" : BufferVar }] }[felts][{ name := "%2" : FeltVar }] ←
+                                        if x0 = (0 : Felt) then (1 : Felt) else (0 : Felt)
+                                    else
+                                      withEqZero x0
+                                        ({
+                                            buffers :=
+                                              ((fun x => Map.empty x)[{ name := "in" : BufferVar }] ←ₘ
+                                                  [[some x0]])[{ name := "data" : BufferVar }] ←ₘ
+                                                [[some (if x0 = (0 : Felt) then (1 : Felt) else (0 : Felt)),
+                                                    some (if x0 = (0 : Felt) then (0 : Felt) else x0⁻¹)]],
+                                            bufferWidths :=
+                                              ((fun x => Map.empty x)[{ name := "data" : BufferVar }] ←ₘ
+                                                  (2 : ℕ))[{ name := "in" : BufferVar }] ←ₘ
+                                                (1 : ℕ),
+                                            constraints := [], cycle := (0 : ℕ),
+                                            felts :=
+                                              (((fun x => Map.empty x)[{ name := "%1" : FeltVar }] ←ₘ
+                                                    x0)[{ name := "%4" : FeltVar }] ←ₘ
+                                                  if x0 = (0 : Felt) then (1 : Felt)
+                                                  else (0 : Felt))[{ name := "%5" : FeltVar }] ←ₘ
+                                                if x0 = (0 : Felt) then (0 : Felt) else x0⁻¹,
+                                            isFailed := false, props := Map.empty,
+                                            vars :=
+                                              [{ name := "in" : BufferVar },
+                                                { name := "data" : BufferVar }] }[felts][{ name := "%2" : FeltVar }] ←
+                                          if x0 = (0 : Felt) then (1 : Felt) else (0 : Felt))).cycle -
+                                  Back.toNat (0 : Back),
+                                (1 : ℕ))))
+                          (Buffer.Idx.data
+                            ((if x0 = (0 : Felt) → False then
+                                    {
+                                        buffers :=
+                                          ((fun x => Map.empty x)[{ name := "in" : BufferVar }] ←ₘ
+                                              [[some x0]])[{ name := "data" : BufferVar }] ←ₘ
+                                            [[some (if x0 = (0 : Felt) then (1 : Felt) else (0 : Felt)),
+                                                some (if x0 = (0 : Felt) then (0 : Felt) else x0⁻¹)]],
+                                        bufferWidths :=
+                                          ((fun x => Map.empty x)[{ name := "data" : BufferVar }] ←ₘ
+                                              (2 : ℕ))[{ name := "in" : BufferVar }] ←ₘ
+                                            (1 : ℕ),
+                                        constraints := [], cycle := (0 : ℕ),
+                                        felts :=
+                                          (((fun x => Map.empty x)[{ name := "%1" : FeltVar }] ←ₘ
+                                                x0)[{ name := "%4" : FeltVar }] ←ₘ
+                                              if x0 = (0 : Felt) then (1 : Felt)
+                                              else (0 : Felt))[{ name := "%5" : FeltVar }] ←ₘ
+                                            if x0 = (0 : Felt) then (0 : Felt) else x0⁻¹,
+                                        isFailed := false, props := Map.empty,
+                                        vars :=
+                                          [{ name := "in" : BufferVar },
+                                            { name := "data" : BufferVar }] }[felts][{ name := "%2" : FeltVar }] ←
+                                      if x0 = (0 : Felt) then (1 : Felt) else (0 : Felt)
+                                  else
+                                    withEqZero x0
+                                      ({
+                                          buffers :=
+                                            ((fun x => Map.empty x)[{ name := "in" : BufferVar }] ←ₘ
+                                                [[some x0]])[{ name := "data" : BufferVar }] ←ₘ
+                                              [[some (if x0 = (0 : Felt) then (1 : Felt) else (0 : Felt)),
+                                                  some (if x0 = (0 : Felt) then (0 : Felt) else x0⁻¹)]],
+                                          bufferWidths :=
+                                            ((fun x => Map.empty x)[{ name := "data" : BufferVar }] ←ₘ
+                                                (2 : ℕ))[{ name := "in" : BufferVar }] ←ₘ
+                                              (1 : ℕ),
+                                          constraints := [], cycle := (0 : ℕ),
+                                          felts :=
+                                            (((fun x => Map.empty x)[{ name := "%1" : FeltVar }] ←ₘ
+                                                  x0)[{ name := "%4" : FeltVar }] ←ₘ
+                                                if x0 = (0 : Felt) then (1 : Felt)
+                                                else (0 : Felt))[{ name := "%5" : FeltVar }] ←ₘ
+                                              if x0 = (0 : Felt) then (0 : Felt) else x0⁻¹,
+                                          isFailed := false, props := Map.empty,
+                                          vars :=
+                                            [{ name := "in" : BufferVar },
+                                              { name := "data" : BufferVar }] }[felts][{ name := "%2" : FeltVar }] ←
+                                        if x0 = (0 : Felt) then (1 : Felt) else (0 : Felt))).cycle -
+                                Back.toNat (0 : Back),
+                              (1 : ℕ))) with
+                      | some x => x
+                      | none =>
+                        panicWithPosWithDecl "Init.Data.Option.BasicAux" "Option.get!" (16 : ℕ) (14 : ℕ)
+                          "value is none")[felts][{ name := "%5" : FeltVar }] ←
+                    x0 *
+                      match
+                        List.get!
+                          (List.get!
+                            (match
+                              State.buffers
+                                (if x0 = (0 : Felt) → False then
+                                  {
+                                      buffers :=
+                                        ((fun x => Map.empty x)[{ name := "in" : BufferVar }] ←ₘ
+                                            [[some x0]])[{ name := "data" : BufferVar }] ←ₘ
+                                          [[some (if x0 = (0 : Felt) then (1 : Felt) else (0 : Felt)),
+                                              some (if x0 = (0 : Felt) then (0 : Felt) else x0⁻¹)]],
+                                      bufferWidths :=
+                                        ((fun x => Map.empty x)[{ name := "data" : BufferVar }] ←ₘ
+                                            (2 : ℕ))[{ name := "in" : BufferVar }] ←ₘ
+                                          (1 : ℕ),
+                                      constraints := [], cycle := (0 : ℕ),
+                                      felts :=
+                                        (((fun x => Map.empty x)[{ name := "%1" : FeltVar }] ←ₘ
+                                              x0)[{ name := "%4" : FeltVar }] ←ₘ
+                                            if x0 = (0 : Felt) then (1 : Felt)
+                                            else (0 : Felt))[{ name := "%5" : FeltVar }] ←ₘ
+                                          if x0 = (0 : Felt) then (0 : Felt) else x0⁻¹,
+                                      isFailed := false, props := Map.empty,
+                                      vars :=
+                                        [{ name := "in" : BufferVar },
+                                          { name := "data" : BufferVar }] }[felts][{ name := "%2" : FeltVar }] ←
+                                    if x0 = (0 : Felt) then (1 : Felt) else (0 : Felt)
+                                else
+                                  withEqZero x0
+                                    ({
+                                        buffers :=
+                                          ((fun x => Map.empty x)[{ name := "in" : BufferVar }] ←ₘ
+                                              [[some x0]])[{ name := "data" : BufferVar }] ←ₘ
+                                            [[some (if x0 = (0 : Felt) then (1 : Felt) else (0 : Felt)),
+                                                some (if x0 = (0 : Felt) then (0 : Felt) else x0⁻¹)]],
+                                        bufferWidths :=
+                                          ((fun x => Map.empty x)[{ name := "data" : BufferVar }] ←ₘ
+                                              (2 : ℕ))[{ name := "in" : BufferVar }] ←ₘ
+                                            (1 : ℕ),
+                                        constraints := [], cycle := (0 : ℕ),
+                                        felts :=
+                                          (((fun x => Map.empty x)[{ name := "%1" : FeltVar }] ←ₘ
+                                                x0)[{ name := "%4" : FeltVar }] ←ₘ
+                                              if x0 = (0 : Felt) then (1 : Felt)
+                                              else (0 : Felt))[{ name := "%5" : FeltVar }] ←ₘ
+                                            if x0 = (0 : Felt) then (0 : Felt) else x0⁻¹,
+                                        isFailed := false, props := Map.empty,
+                                        vars :=
+                                          [{ name := "in" : BufferVar },
+                                            { name := "data" : BufferVar }] }[felts][{ name := "%2" : FeltVar }] ←
+                                      if x0 = (0 : Felt) then (1 : Felt) else (0 : Felt)))
+                                { name := "data" : BufferVar } with
+                            | some x => x
+                            | none =>
+                              panicWithPosWithDecl "Init.Data.Option.BasicAux" "Option.get!" (16 : ℕ) (14 : ℕ)
+                                "value is none")
+                            (Buffer.Idx.time
+                              ((if x0 = (0 : Felt) → False then
+                                      {
+                                          buffers :=
+                                            ((fun x => Map.empty x)[{ name := "in" : BufferVar }] ←ₘ
+                                                [[some x0]])[{ name := "data" : BufferVar }] ←ₘ
+                                              [[some (if x0 = (0 : Felt) then (1 : Felt) else (0 : Felt)),
+                                                  some (if x0 = (0 : Felt) then (0 : Felt) else x0⁻¹)]],
+                                          bufferWidths :=
+                                            ((fun x => Map.empty x)[{ name := "data" : BufferVar }] ←ₘ
+                                                (2 : ℕ))[{ name := "in" : BufferVar }] ←ₘ
+                                              (1 : ℕ),
+                                          constraints := [], cycle := (0 : ℕ),
+                                          felts :=
+                                            (((fun x => Map.empty x)[{ name := "%1" : FeltVar }] ←ₘ
+                                                  x0)[{ name := "%4" : FeltVar }] ←ₘ
+                                                if x0 = (0 : Felt) then (1 : Felt)
+                                                else (0 : Felt))[{ name := "%5" : FeltVar }] ←ₘ
+                                              if x0 = (0 : Felt) then (0 : Felt) else x0⁻¹,
+                                          isFailed := false, props := Map.empty,
+                                          vars :=
+                                            [{ name := "in" : BufferVar },
+                                              { name := "data" : BufferVar }] }[felts][{ name := "%2" : FeltVar }] ←
+                                        if x0 = (0 : Felt) then (1 : Felt) else (0 : Felt)
+                                    else
+                                      withEqZero x0
+                                        ({
+                                            buffers :=
+                                              ((fun x => Map.empty x)[{ name := "in" : BufferVar }] ←ₘ
+                                                  [[some x0]])[{ name := "data" : BufferVar }] ←ₘ
+                                                [[some (if x0 = (0 : Felt) then (1 : Felt) else (0 : Felt)),
+                                                    some (if x0 = (0 : Felt) then (0 : Felt) else x0⁻¹)]],
+                                            bufferWidths :=
+                                              ((fun x => Map.empty x)[{ name := "data" : BufferVar }] ←ₘ
+                                                  (2 : ℕ))[{ name := "in" : BufferVar }] ←ₘ
+                                                (1 : ℕ),
+                                            constraints := [], cycle := (0 : ℕ),
+                                            felts :=
+                                              (((fun x => Map.empty x)[{ name := "%1" : FeltVar }] ←ₘ
+                                                    x0)[{ name := "%4" : FeltVar }] ←ₘ
+                                                  if x0 = (0 : Felt) then (1 : Felt)
+                                                  else (0 : Felt))[{ name := "%5" : FeltVar }] ←ₘ
+                                                if x0 = (0 : Felt) then (0 : Felt) else x0⁻¹,
+                                            isFailed := false, props := Map.empty,
+                                            vars :=
+                                              [{ name := "in" : BufferVar },
+                                                { name := "data" : BufferVar }] }[felts][{ name := "%2" : FeltVar }] ←
+                                          if x0 = (0 : Felt) then (1 : Felt) else (0 : Felt))).cycle -
+                                  Back.toNat (0 : Back),
+                                (1 : ℕ))))
+                          (Buffer.Idx.data
+                            ((if x0 = (0 : Felt) → False then
+                                    {
+                                        buffers :=
+                                          ((fun x => Map.empty x)[{ name := "in" : BufferVar }] ←ₘ
+                                              [[some x0]])[{ name := "data" : BufferVar }] ←ₘ
+                                            [[some (if x0 = (0 : Felt) then (1 : Felt) else (0 : Felt)),
+                                                some (if x0 = (0 : Felt) then (0 : Felt) else x0⁻¹)]],
+                                        bufferWidths :=
+                                          ((fun x => Map.empty x)[{ name := "data" : BufferVar }] ←ₘ
+                                              (2 : ℕ))[{ name := "in" : BufferVar }] ←ₘ
+                                            (1 : ℕ),
+                                        constraints := [], cycle := (0 : ℕ),
+                                        felts :=
+                                          (((fun x => Map.empty x)[{ name := "%1" : FeltVar }] ←ₘ
+                                                x0)[{ name := "%4" : FeltVar }] ←ₘ
+                                              if x0 = (0 : Felt) then (1 : Felt)
+                                              else (0 : Felt))[{ name := "%5" : FeltVar }] ←ₘ
+                                            if x0 = (0 : Felt) then (0 : Felt) else x0⁻¹,
+                                        isFailed := false, props := Map.empty,
+                                        vars :=
+                                          [{ name := "in" : BufferVar },
+                                            { name := "data" : BufferVar }] }[felts][{ name := "%2" : FeltVar }] ←
+                                      if x0 = (0 : Felt) then (1 : Felt) else (0 : Felt)
+                                  else
+                                    withEqZero x0
+                                      ({
+                                          buffers :=
+                                            ((fun x => Map.empty x)[{ name := "in" : BufferVar }] ←ₘ
+                                                [[some x0]])[{ name := "data" : BufferVar }] ←ₘ
+                                              [[some (if x0 = (0 : Felt) then (1 : Felt) else (0 : Felt)),
+                                                  some (if x0 = (0 : Felt) then (0 : Felt) else x0⁻¹)]],
+                                          bufferWidths :=
+                                            ((fun x => Map.empty x)[{ name := "data" : BufferVar }] ←ₘ
+                                                (2 : ℕ))[{ name := "in" : BufferVar }] ←ₘ
+                                              (1 : ℕ),
+                                          constraints := [], cycle := (0 : ℕ),
+                                          felts :=
+                                            (((fun x => Map.empty x)[{ name := "%1" : FeltVar }] ←ₘ
+                                                  x0)[{ name := "%4" : FeltVar }] ←ₘ
+                                                if x0 = (0 : Felt) then (1 : Felt)
+                                                else (0 : Felt))[{ name := "%5" : FeltVar }] ←ₘ
+                                              if x0 = (0 : Felt) then (0 : Felt) else x0⁻¹,
+                                          isFailed := false, props := Map.empty,
+                                          vars :=
+                                            [{ name := "in" : BufferVar },
+                                              { name := "data" : BufferVar }] }[felts][{ name := "%2" : FeltVar }] ←
+                                        if x0 = (0 : Felt) then (1 : Felt) else (0 : Felt))).cycle -
+                                Back.toNat (0 : Back),
+                              (1 : ℕ))) with
+                      | some x => x
+                      | none =>
+                        panicWithPosWithDecl "Init.Data.Option.BasicAux" "Option.get!" (16 : ℕ) (14 : ℕ)
+                          "value is none")[felts][{ name := "%6" : FeltVar }] ←
+                  (x0 *
+                      match
+                        List.get!
+                          (List.get!
+                            (match
+                              State.buffers
+                                (if x0 = (0 : Felt) → False then
+                                  {
+                                      buffers :=
+                                        ((fun x => Map.empty x)[{ name := "in" : BufferVar }] ←ₘ
+                                            [[some x0]])[{ name := "data" : BufferVar }] ←ₘ
+                                          [[some (if x0 = (0 : Felt) then (1 : Felt) else (0 : Felt)),
+                                              some (if x0 = (0 : Felt) then (0 : Felt) else x0⁻¹)]],
+                                      bufferWidths :=
+                                        ((fun x => Map.empty x)[{ name := "data" : BufferVar }] ←ₘ
+                                            (2 : ℕ))[{ name := "in" : BufferVar }] ←ₘ
+                                          (1 : ℕ),
+                                      constraints := [], cycle := (0 : ℕ),
+                                      felts :=
+                                        (((fun x => Map.empty x)[{ name := "%1" : FeltVar }] ←ₘ
+                                              x0)[{ name := "%4" : FeltVar }] ←ₘ
+                                            if x0 = (0 : Felt) then (1 : Felt)
+                                            else (0 : Felt))[{ name := "%5" : FeltVar }] ←ₘ
+                                          if x0 = (0 : Felt) then (0 : Felt) else x0⁻¹,
+                                      isFailed := false, props := Map.empty,
+                                      vars :=
+                                        [{ name := "in" : BufferVar },
+                                          { name := "data" : BufferVar }] }[felts][{ name := "%2" : FeltVar }] ←
+                                    if x0 = (0 : Felt) then (1 : Felt) else (0 : Felt)
+                                else
+                                  withEqZero x0
+                                    ({
+                                        buffers :=
+                                          ((fun x => Map.empty x)[{ name := "in" : BufferVar }] ←ₘ
+                                              [[some x0]])[{ name := "data" : BufferVar }] ←ₘ
+                                            [[some (if x0 = (0 : Felt) then (1 : Felt) else (0 : Felt)),
+                                                some (if x0 = (0 : Felt) then (0 : Felt) else x0⁻¹)]],
+                                        bufferWidths :=
+                                          ((fun x => Map.empty x)[{ name := "data" : BufferVar }] ←ₘ
+                                              (2 : ℕ))[{ name := "in" : BufferVar }] ←ₘ
+                                            (1 : ℕ),
+                                        constraints := [], cycle := (0 : ℕ),
+                                        felts :=
+                                          (((fun x => Map.empty x)[{ name := "%1" : FeltVar }] ←ₘ
+                                                x0)[{ name := "%4" : FeltVar }] ←ₘ
+                                              if x0 = (0 : Felt) then (1 : Felt)
+                                              else (0 : Felt))[{ name := "%5" : FeltVar }] ←ₘ
+                                            if x0 = (0 : Felt) then (0 : Felt) else x0⁻¹,
+                                        isFailed := false, props := Map.empty,
+                                        vars :=
+                                          [{ name := "in" : BufferVar },
+                                            { name := "data" : BufferVar }] }[felts][{ name := "%2" : FeltVar }] ←
+                                      if x0 = (0 : Felt) then (1 : Felt) else (0 : Felt)))
+                                { name := "data" : BufferVar } with
+                            | some x => x
+                            | none =>
+                              panicWithPosWithDecl "Init.Data.Option.BasicAux" "Option.get!" (16 : ℕ) (14 : ℕ)
+                                "value is none")
+                            (Buffer.Idx.time
+                              ((if x0 = (0 : Felt) → False then
+                                      {
+                                          buffers :=
+                                            ((fun x => Map.empty x)[{ name := "in" : BufferVar }] ←ₘ
+                                                [[some x0]])[{ name := "data" : BufferVar }] ←ₘ
+                                              [[some (if x0 = (0 : Felt) then (1 : Felt) else (0 : Felt)),
+                                                  some (if x0 = (0 : Felt) then (0 : Felt) else x0⁻¹)]],
+                                          bufferWidths :=
+                                            ((fun x => Map.empty x)[{ name := "data" : BufferVar }] ←ₘ
+                                                (2 : ℕ))[{ name := "in" : BufferVar }] ←ₘ
+                                              (1 : ℕ),
+                                          constraints := [], cycle := (0 : ℕ),
+                                          felts :=
+                                            (((fun x => Map.empty x)[{ name := "%1" : FeltVar }] ←ₘ
+                                                  x0)[{ name := "%4" : FeltVar }] ←ₘ
+                                                if x0 = (0 : Felt) then (1 : Felt)
+                                                else (0 : Felt))[{ name := "%5" : FeltVar }] ←ₘ
+                                              if x0 = (0 : Felt) then (0 : Felt) else x0⁻¹,
+                                          isFailed := false, props := Map.empty,
+                                          vars :=
+                                            [{ name := "in" : BufferVar },
+                                              { name := "data" : BufferVar }] }[felts][{ name := "%2" : FeltVar }] ←
+                                        if x0 = (0 : Felt) then (1 : Felt) else (0 : Felt)
+                                    else
+                                      withEqZero x0
+                                        ({
+                                            buffers :=
+                                              ((fun x => Map.empty x)[{ name := "in" : BufferVar }] ←ₘ
+                                                  [[some x0]])[{ name := "data" : BufferVar }] ←ₘ
+                                                [[some (if x0 = (0 : Felt) then (1 : Felt) else (0 : Felt)),
+                                                    some (if x0 = (0 : Felt) then (0 : Felt) else x0⁻¹)]],
+                                            bufferWidths :=
+                                              ((fun x => Map.empty x)[{ name := "data" : BufferVar }] ←ₘ
+                                                  (2 : ℕ))[{ name := "in" : BufferVar }] ←ₘ
+                                                (1 : ℕ),
+                                            constraints := [], cycle := (0 : ℕ),
+                                            felts :=
+                                              (((fun x => Map.empty x)[{ name := "%1" : FeltVar }] ←ₘ
+                                                    x0)[{ name := "%4" : FeltVar }] ←ₘ
+                                                  if x0 = (0 : Felt) then (1 : Felt)
+                                                  else (0 : Felt))[{ name := "%5" : FeltVar }] ←ₘ
+                                                if x0 = (0 : Felt) then (0 : Felt) else x0⁻¹,
+                                            isFailed := false, props := Map.empty,
+                                            vars :=
+                                              [{ name := "in" : BufferVar },
+                                                { name := "data" : BufferVar }] }[felts][{ name := "%2" : FeltVar }] ←
+                                          if x0 = (0 : Felt) then (1 : Felt) else (0 : Felt))).cycle -
+                                  Back.toNat (0 : Back),
+                                (1 : ℕ))))
+                          (Buffer.Idx.data
+                            ((if x0 = (0 : Felt) → False then
+                                    {
+                                        buffers :=
+                                          ((fun x => Map.empty x)[{ name := "in" : BufferVar }] ←ₘ
+                                              [[some x0]])[{ name := "data" : BufferVar }] ←ₘ
+                                            [[some (if x0 = (0 : Felt) then (1 : Felt) else (0 : Felt)),
+                                                some (if x0 = (0 : Felt) then (0 : Felt) else x0⁻¹)]],
+                                        bufferWidths :=
+                                          ((fun x => Map.empty x)[{ name := "data" : BufferVar }] ←ₘ
+                                              (2 : ℕ))[{ name := "in" : BufferVar }] ←ₘ
+                                            (1 : ℕ),
+                                        constraints := [], cycle := (0 : ℕ),
+                                        felts :=
+                                          (((fun x => Map.empty x)[{ name := "%1" : FeltVar }] ←ₘ
+                                                x0)[{ name := "%4" : FeltVar }] ←ₘ
+                                              if x0 = (0 : Felt) then (1 : Felt)
+                                              else (0 : Felt))[{ name := "%5" : FeltVar }] ←ₘ
+                                            if x0 = (0 : Felt) then (0 : Felt) else x0⁻¹,
+                                        isFailed := false, props := Map.empty,
+                                        vars :=
+                                          [{ name := "in" : BufferVar },
+                                            { name := "data" : BufferVar }] }[felts][{ name := "%2" : FeltVar }] ←
+                                      if x0 = (0 : Felt) then (1 : Felt) else (0 : Felt)
+                                  else
+                                    withEqZero x0
+                                      ({
+                                          buffers :=
+                                            ((fun x => Map.empty x)[{ name := "in" : BufferVar }] ←ₘ
+                                                [[some x0]])[{ name := "data" : BufferVar }] ←ₘ
+                                              [[some (if x0 = (0 : Felt) then (1 : Felt) else (0 : Felt)),
+                                                  some (if x0 = (0 : Felt) then (0 : Felt) else x0⁻¹)]],
+                                          bufferWidths :=
+                                            ((fun x => Map.empty x)[{ name := "data" : BufferVar }] ←ₘ
+                                                (2 : ℕ))[{ name := "in" : BufferVar }] ←ₘ
+                                              (1 : ℕ),
+                                          constraints := [], cycle := (0 : ℕ),
+                                          felts :=
+                                            (((fun x => Map.empty x)[{ name := "%1" : FeltVar }] ←ₘ
+                                                  x0)[{ name := "%4" : FeltVar }] ←ₘ
+                                                if x0 = (0 : Felt) then (1 : Felt)
+                                                else (0 : Felt))[{ name := "%5" : FeltVar }] ←ₘ
+                                              if x0 = (0 : Felt) then (0 : Felt) else x0⁻¹,
+                                          isFailed := false, props := Map.empty,
+                                          vars :=
+                                            [{ name := "in" : BufferVar },
+                                              { name := "data" : BufferVar }] }[felts][{ name := "%2" : FeltVar }] ←
+                                        if x0 = (0 : Felt) then (1 : Felt) else (0 : Felt))).cycle -
+                                Back.toNat (0 : Back),
+                              (1 : ℕ))) with
+                      | some x => x
+                      | none =>
+                        panicWithPosWithDecl "Init.Data.Option.BasicAux" "Option.get!" (16 : ℕ) (14 : ℕ)
+                          "value is none") -
+                    (1 : Felt)))
+            { name := "data" : BufferVar }) with
+      | [] => panicWithPosWithDecl "Init.Data.List.BasicAux" "List.getLast!" (63 : ℕ) (13 : ℕ) "empty list"
+      | a :: as => List.getLast (a :: as) (_ : a :: as = [] → List.noConfusionType False (a :: as) []) =
+      [y0, y1]  := by
+    rewrite [part2_cumulative_wp]
+    unfold part2_state_update
+    unfold part2_state
+    try simplify_get_hack
+    MLIR_states_updates
+    -- 0 withEqZeros
+    -- rewrite [withEqZero_def]
+    -- MLIR_states_updates
+    unfold part2_drops
+    -- 7 drops
+    simp only [State.drop_update_swap, State.drop_update_same]
+    rewrite [State.dropFelts]
+    simp only [State.dropFelts_buffers, State.dropFelts_bufferWidths, State.dropFelts_constraints, State.dropFelts_cycle, State.dropFelts_felts, State.dropFelts_isFailed, State.dropFelts_props, State.dropFelts_vars]
+    simp only [Map.drop_base, ne_eq, Map.update_drop_swap, Map.update_drop]
+    -- 0 sets
+    -- rewrite [Map.drop_of_updates]
+    -- simp only [Map.drop_base, ne_eq, Map.update_drop_swap, Map.update_drop]
+    unfold Code.getReturn
+    simp only
+    simp [Map.update_get_wobbly, List.getLast!]
 end Risc0.IsZero.Witness.WP
